WIP

backend/MachC.v
@@ -247,6 +247,28 @@ Definition get_mem (st: state): mem :=
   | Returnstate _ _ m0 => m0
   end.
 
+
+Inductive store_arguments (m0: mem) (rs: regset) (vs: list val) (sg: signature) (m2: mem): Prop :=
+| store_arguments_intro
+    m1 blk
+    (ALC: Mem.alloc m0 0 (size_arguments sg) = (m1, blk))
+    (VALS: extcall_arguments rs m2 (Vptr blk Ptrofs.zero true) sg vs)
+    (UNCH: Mem.unchanged_on (fun b ofs => if eq_block b blk
+                                          then ~ (0 <= ofs < 4 * size_arguments sg)
+                                          else True) m1 m2)
+    (NB: m1.(Mem.nextblock) = m2.(Mem.nextblock))
+    (PERM: Mem.range_perm m2 blk 0 (4 * size_arguments sg) Cur Freeable)
+.
+
+Lemma store_arguments_progress
+      m0 vs sg
+  :
+    exists rs m2, <<STR: store_arguments m0 rs vs sg m2>>
+.
+Proof.
+  admit "".
+Qed.
+
 Section MODSEM.
 
   Variable rao: function -> code -> ptrofs -> Prop.
@@ -275,7 +297,7 @@ Section MODSEM.
       (SIG: exists skd, skenv_link.(Genv.find_funct) fptr = Some skd /\ SkEnv.get_sig skd = sg)
       (VALS: extcall_arguments rs m0 (parent_sp stack) sg vs)
       (RSP: (parent_sp stack) = Vptr blk ofs true)
-      (FREE: Mem.free m0 blk ofs.(Ptrofs.unsigned) (1 + ofs.(Ptrofs.unsigned) + (size_arguments sg)) = Some m1)
+      (FREE: Mem.free m0 blk ofs.(Ptrofs.unsigned) (ofs.(Ptrofs.unsigned) + 4 * (size_arguments sg)) = Some m1)
       init_rs init_sg
     :
       at_external skenv_link (mkstate init_rs init_sg (Callstate stack fptr rs m0)) (Args.mk fptr vs m1)
@@ -284,24 +306,22 @@ Section MODSEM.
   Inductive initial_frame (args: Args.t)
     : state -> Prop :=
   | initial_frame_intro
-      fd m0 m1 rs blk sg
+      fd m0 rs sg
       (SIG: sg = fd.(fn_sig))
       (FINDF: Genv.find_funct ge args.(Args.fptr) = Some (Internal fd))
-      (ALLOC: Mem.alloc args.(Args.m) 0 (size_arguments sg) = (m0, blk))
-      (STORE: extcall_arguments rs m1 (Vptr blk Ptrofs.zero true) sg args.(Args.vs)
-              /\ Mem.unchanged_on (fun b ofs => if eq_block b blk
-                                                then ~ (0 <= ofs < 4 * size_arguments sg)
-                                                else True) m0 m1
-              /\ Mem.range_perm m1 blk 0 (4 * size_arguments sg) Cur Freeable)
+      (STORE: store_arguments args.(Args.m) rs args.(Args.vs) sg m0)
       (PTRFREE: forall
           mr
-          (NOTIN: Loc.notin (R mr) (regs_of_rpairs (loc_arguments sg)))
+          (* (NOTIN: Loc.notin (R mr) (regs_of_rpairs (loc_arguments sg))) *)
+          (NOTIN: ~In (R mr) (regs_of_rpairs (loc_arguments sg)))
         ,
           <<PTRFREE: ~ is_real_ptr (rs mr)>>)
+      (SZ: 4 * size_arguments sg <= Ptrofs.modulus)
     :
       initial_frame args (mkstate rs sg
-                                  (Callstate [dummy_stack (Vptr blk Ptrofs.zero true) Vundef]
-                                             args.(Args.fptr) rs m1))
+                                  (Callstate [dummy_stack
+                                                (Vptr args.(Args.m).(Mem.nextblock) Ptrofs.zero true) Vundef]
+                                             args.(Args.fptr) rs m0))
   .
 
   Inductive final_frame: state -> Retv.t -> Prop :=
@@ -323,7 +343,7 @@ Section MODSEM.
       (SIG: exists skd, skenv_link.(Genv.find_funct) fptr = Some skd /\ SkEnv.get_sig skd = sg)
       (REGSET: ls1 = (set_pair (loc_result sg) retv.(Retv.v) (regset_after_external ls0)))
       (RSP: (parent_sp stack) = Vptr blk ofs true)
-      (UNFREE: Mem_unfree m0 blk ofs.(Ptrofs.unsigned) (1 + ofs.(Ptrofs.unsigned) + (size_arguments sg)) = Some m1)
+      (UNFREE: Mem_unfree m0 blk ofs.(Ptrofs.unsigned) (ofs.(Ptrofs.unsigned) + 4 * (size_arguments sg)) = Some m1)
     :
       after_external (mkstate init_rs init_sg (Callstate stack fptr ls0 m0))
                      retv
